theories/examples/generative.v
@@ -1,0 +1,252 @@
+(* ReLoC -- Relational logic for fine-grained concurrency *)
+(** Examples from "State-Dependent Represenation Independence" by A.
+Ahmed, D. Dreyer, A. Rossberg.
+
+Those are mostly "generative ADTs". *)
+From iris.proofmode Require Import tactics.
+From iris.heap_lang.lib Require Export par.
+From reloc Require Export proofmode prelude.bijections.
+From reloc.examples Require Export counter lock.
+From reloc.typing Require Export interp soundness.
+
+(** Using references for name generation *)
+(* ∃ α. (1 → α) × (α → α → 2)                     *)
+(*       ^ new name  ^                            *)
+(*                   | compare names for equality *)
+Definition nameGenTy : type := TExists (TProd (TArrow TUnit (TVar 0))
+                                              (TArrow (TVar 0) (TArrow (TVar 0) TBool)))%nat.
+
+(* TODO: cannot be a value *)
+Definition nameGen1 : expr :=
+  (λ: <>, ref #()
+  ,λ: "y" "z", "y" = "z").
+
+Definition nameGen2 : expr :=
+  let: "x" := ref #0 in
+  (λ: <>, FG_increment "x";; !"x"
+  ,λ: "y" "z", "y" = "z").
+
+Section namegen_refinement.
+  Context `{relocG Σ, PrePBijG loc nat Σ}.
+
+  Program Definition ngR (γ : gname) : lty2 Σ := Lty2 (λ v1 v2,
+   ∃ (l : loc) (n : nat), ⌜v1 = #l%V⌝ ∗ ⌜v2 = #n⌝
+                         ∗ inBij γ l n)%I.
+
+  Definition ng_Inv (γ : gname) (c : loc) : iProp Σ :=
+    (∃ (n : nat) (L : gset (loc * nat)),
+        BIJ γ L ∗ c ↦ₛ #n
+     ∗  [∗ set] lk ∈ L, match lk with
+                        | (l, k) => l ↦ #() ∗ ⌜k ≤ n⌝%nat
+                        end)%I.
+
+  Lemma nameGen_ref1 :
+    REL nameGen1 << nameGen2 : ∃ α, (() → α) × (α → α → lty2_bool).
+  Proof.
+    unlock nameGen1 nameGen2.
+    rel_alloc_r c as "Hc".
+    iMod alloc_empty_bij as (γ) "HB".
+    pose (N:=relocN.@"ng").
+    iMod (inv_alloc N _ (ng_Inv γ c) with "[-]") as "#Hinv".
+    { iNext. iExists 0%nat, ∅. iFrame.
+      by rewrite big_sepS_empty. }
+    iApply (refines_exists (ngR γ)).
+    do 2 rel_pure_r.
+    iApply refines_pair.
+    - (* New name *)
+      rel_pure_l. rel_pure_r.
+      iApply refines_arrow.
+      iAlways. iIntros (? ?) "/= _".
+      rel_pure_l. rel_pure_r.
+      rel_alloc_l_atomic.
+      iInv N as (n L) "(HB & Hc & HL)" "Hcl".
+      iModIntro. iNext. iIntros (l') "Hl'".
+      rel_apply_r (FG_increment_r with "Hc").
+      iIntros "Hc". repeat rel_pure_r. rel_load_r.
+      iAssert (⌜(∃ y, (l', y) ∈ L) → False⌝)%I with "[HL Hl']" as %Hl'.
+      { iIntros (Hy). destruct Hy as [y Hy].
+        rewrite (big_sepS_elem_of _ L (l',y) Hy).
+        iDestruct "HL" as "[Hl _]".
+        iDestruct (gen_heap.mapsto_valid_2 with "Hl Hl'") as %Hfoo.
+        compute in Hfoo. eauto. }
+      iAssert (⌜(∃ x, (x, S n) ∈ L) → False⌝)%I with "[HL]" as %Hc.
+      { iIntros (Hx). destruct Hx as [x Hy].
+        rewrite (big_sepS_elem_of _ L (x,S n) Hy).
+        iDestruct "HL" as "[_ %]". omega. }
+      iMod (bij_alloc_alt _ _ γ _ l' (S n) with "HB") as "[HB #Hl'n]"; auto.
+      iMod ("Hcl" with "[-]").
+      { iNext.
+        replace (Z.of_nat n + 1) with (Z.of_nat (n + 1)); last lia.
+        iExists _,_; iFrame "Hc HB".
+        rewrite big_sepS_insert; last by naive_solver.
+        iFrame. iSplit; first (iPureIntro; lia).
+        iApply (big_sepS_mono _ _ L with "HL").
+        intros [l x] Hlx. apply bi.sep_mono_r, bi.pure_mono. lia. }
+      rel_values. iModIntro.
+      replace (Z.of_nat n + 1) with (Z.of_nat (S n)); last lia.
+      iExists l', (S n)%nat; eauto.
+    - (* Name comparison *)
+      rel_pure_l. rel_pure_r.
+      iApply refines_arrow_val.
+      iAlways. iIntros (? ?) "/= #Hv".
+      iDestruct "Hv" as (l n) "(% & % & #Hln)". simplify_eq.
+      do 2 rel_pure_l. do 2 rel_pure_r.
+      iApply refines_arrow_val.
+      iAlways. iIntros (? ?) "/= #Hv".
+      iDestruct "Hv" as (l' n') "(% & % & #Hl'n')". simplify_eq.
+      do 2 rel_pure_l. do 2 rel_pure_r.
+      iInv N as (m L) "(>HB & >Hc & HL)" "Hcl".
+      iDestruct (bij_agree with "HB Hln Hl'n'") as %Hag.
+      destruct (decide (l = l')) as [->|Hll].
+      + assert (n = n') as -> by (apply Hag; auto).
+        case_decide; last by contradiction.
+        iMod ("Hcl" with "[-]") as "_".
+        { iNext. iExists _,_; iFrame. }
+        rewrite !bool_decide_true //.
+        rel_values.
+      + assert (n ≠ n') as Hnn'.
+        { intros Hnn. apply Hll. by apply Hag. }
+        case_decide; first by simplify_eq/=.
+        iMod ("Hcl" with "[-]") as "_".
+        { iNext. iExists _,_; iFrame. }
+        rewrite !bool_decide_false //; first rel_values.
+        inversion 1; simplify_eq/=.
+  Qed.
+End namegen_refinement.
+
+(** A type of cells -- basically an abstract type of references. *)
+(* ∀ α, ∃ β, (α → β) × (β → α) × (β → α → ())  *)
+Definition cellτ : type :=
+  TForall (TExists (TProd (TProd (TArrow (TVar 1) (TVar 0))
+                                 (TArrow (TVar 0) (TVar 1)))
+                                 (TArrow (TVar 0) (TArrow (TVar 1) TUnit))))%nat.
+(* TODO: should these be values? *)
+Definition cell1 : expr :=
+  (Λ: (λ: "x", ref "x", λ: "r", !"r", λ: "r" "x", "r" <- "x")).
+
+Definition cell2 : expr :=
+  Λ: ( λ: "x",
+       let: "r1" := ref #false in
+       let: "r2" := ref "x" in
+       let: "r3" := ref "x" in
+       let: "lk" := newlock #() in
+       ("r1", "r2", "r3", "lk")
+     ,  λ: "r", let: "l" := (Snd "r") in
+                acquire "l";;
+                let: "v" :=
+                   if: !(Fst (Fst (Fst "r")))
+                   then !(Snd (Fst "r"))
+                   else !(Snd (Fst (Fst "r"))) in
+                release "l";;
+                "v"
+     , λ: "r" "x", let: "l" := (Snd "r") in
+                   acquire "l";;
+                   (if: !(Fst (Fst (Fst "r")))
+                    then (Snd (Fst (Fst "r"))) <- "x";;
+                         (Fst (Fst (Fst "r"))) <- #false
+                    else (Snd (Fst "r")) <- "x";;
+                         (Fst (Fst (Fst "r"))) <- #true);;
+                   release "l").
+
+Section cell_refinement.
+  Context `{relocG Σ, lockG Σ}.
+
+  Definition lockR (R : lty2 Σ) (r1 r2 r3 r : loc) : iProp Σ :=
+    (∃ (a b c : val), r ↦ₛ a ∗ r2 ↦ b ∗ r3 ↦ c ∗
+     ( (r1 ↦ #true ∗ R c a)
+     ∨ (r1 ↦ #false ∗ R b a)))%I.
+
+  Definition cellInt (R : lty2 Σ) (r1 r2 r3 l r : loc) : iProp Σ :=
+    (∃ γ N, is_lock N γ #l (lockR R r1 r2 r3 r))%I.
+
+  Program Definition cellR (R : lty2 Σ) : lty2 Σ := Lty2 (λ v1 v2,
+    ∃ r1 r2 r3 l r : loc, ⌜v1 = (#r1, #r2, #r3, #l)%V⌝ ∗ ⌜v2 = #r⌝
+     ∗ cellInt R r1 r2 r3 l r)%I.
+
+  Lemma cell2_cell1_refinement :
+    REL cell2 << cell1 : ∀ α, ∃ β, (α → β) × (β → α) × (β → α → ()).
+  Proof.
+    unlock cell2 cell1.
+    (* TODO: this uuugly *)
+    pose (τ := (TExists (TProd (TProd (TArrow (TVar 1) (TVar 0))
+                                 (TArrow (TVar 0) (TVar 1)))
+                                 (TArrow (TVar 0) (TArrow (TVar 1) TUnit))))%nat).
+    iPoseProof (bin_log_related_tlam [] ∅ _ _ τ) as "H".
+    iSpecialize ("H" with "[]"); last first.
+    { rewrite /bin_log_related.
+      iSpecialize ("H" $! ∅ with "[]").
+      - rewrite fmap_empty. iApply env_ltyped2_empty.
+      - rewrite !fmap_empty !subst_map_empty.
+        iSimpl in "H". iApply "H". }
+    iIntros (R) "!#".
+    iApply (bin_log_related_pack (cellR R)).
+    iIntros (vs) "Hvs". rewrite !fmap_empty env_ltyped2_empty_inv.
+    iDestruct "Hvs" as %->. rewrite !fmap_empty !subst_map_empty.
+    iSimpl. repeat iApply refines_pair.
+    - (* New cell *)
+      rel_pure_l. rel_pure_r.
+      iApply refines_arrow_val.
+      iAlways. iIntros (v1 v2) "/= #Hv".
+      rel_let_l. rel_let_r.
+      rel_alloc_r r as "Hr".
+
+      rel_alloc_l r1 as "Hr1". repeat rel_pure_l.
+      rel_alloc_l r2 as "Hr2". repeat rel_pure_l.
+      rel_alloc_l r3 as "Hr3". repeat rel_pure_l.
+
+      pose (N:=relocN.@(r1,r)).
+      rel_apply_l (refines_newlock_l N (lockR R r1 r2 r3 r)%I with "[-]").
+      { iExists _,_,_. iFrame.
+        iRight. by iFrame. }
+
+      iNext. iIntros (lk γl) "#Hlk".
+      repeat rel_pure_l. rel_values. iModIntro.
+      iExists _,_,_,_,_. repeat iSplit; eauto.
+      iExists _,_. by iFrame.
+    - (* Read cell *)
+      rel_pure_l. rel_pure_r.
+      iApply refines_arrow_val.
+      iAlways. iIntros (v1 v2) "/=".
+      iDestruct 1 as (r1 r2 r3 l r) "[% [% #Hrs]]". simplify_eq.
+      repeat rel_pure_l.
+      rewrite /cellInt. iDestruct "Hrs" as (γlk N) "#Hlk".
+      rel_apply_l (refines_acquire_l with "Hlk"); first auto.
+      iNext. iIntros "Htok".
+      rewrite /lockR. iDestruct 1 as (a b c) "(Hr & Hr2 & Hr3 & Hr1)".
+      repeat rel_pure_l.
+      rel_let_r. rel_load_r.
+      iDestruct "Hr1" as "[[Hr1 #Ha] | [Hr1 #Ha]]";
+        rel_load_l; repeat rel_pure_l; rel_load_l; repeat rel_pure_l.
+      + rel_apply_l (refines_release_l with "Hlk Htok [-]"); auto.
+        { iExists a,b,c; iFrame. iLeft; by iFrame. }
+        iNext. repeat rel_pure_l. rel_values.
+      + rel_apply_l (refines_release_l with "Hlk Htok [-]"); auto.
+        { iExists _,_,_; iFrame. iRight; by iFrame. }
+        iNext. repeat rel_pure_l. rel_values.
+    - (* Insert cell *)
+      rel_pure_l. rel_pure_r.
+      iApply refines_arrow_val.
+      iAlways. iIntros (v1 v2) "/=".
+      iDestruct 1 as (r1 r2 r3 l r) "[% [% #Hrs]]". simplify_eq.
+      repeat rel_pure_l. repeat rel_pure_r.
+      iApply refines_arrow_val.
+      iAlways. iIntros (v1 v2) "/= #Hv".
+      repeat rel_pure_l. repeat rel_pure_r.
+      rewrite /cellInt. iDestruct "Hrs" as (γlk N) "#Hlk".
+      rel_apply_l (refines_acquire_l with "Hlk"); first auto.
+      iNext. iIntros "Htok".
+      rewrite /lockR. iDestruct 1 as (a b c) "(Hr & Hr2 & Hr3 & Hr1)".
+      repeat rel_pure_l. rel_store_r.
+      iDestruct "Hr1" as "[[Hr1 #Ha] | [Hr1 #Ha]]";
+        rel_load_l;
+        repeat rel_pure_l; rel_store_l; repeat rel_pure_l;
+        repeat rel_pure_l; rel_store_l; repeat rel_pure_l.
+      + rel_apply_l (refines_release_l with "Hlk Htok [-]"); auto.
+        { iExists _,_,_; iFrame. iRight; by iFrame. }
+        iNext. rel_values.
+      + rel_apply_l (refines_release_l with "Hlk Htok [-]"); auto.
+        { iExists _,_,_; iFrame. iLeft; by iFrame. }
+        iNext. rel_values.
+    Qed.
+End cell_refinement.
+
